interface for FStar.UInt

ulib/FStar.UInt.fst
@@ -22,22 +22,6 @@ open FStar.Mul
 open FStar.BitVector
 open FStar.Math.Lemmas
 
-#push-options "--max_fuel 0 --max_ifuel 0"
-
-val pow2_values: x:nat -> Lemma
-  (let p = pow2 x in
-   match x with
-   | 0  -> p=1
-   | 1  -> p=2
-   | 8  -> p=256
-   | 16 -> p=65536
-   | 31 -> p=2147483648
-   | 32 -> p=4294967296
-   | 63 -> p=9223372036854775808
-   | 64 -> p=18446744073709551616
-   | 128 -> p=0x100000000000000000000000000000000
-   | _  -> True)
-  [SMTPat (pow2 x)]
 let pow2_values x =
    match x with
    | 0  -> assert_norm (pow2 0 == 1)
@@ -51,198 +35,35 @@ let pow2_values x =
    | 128 -> assert_norm (pow2 128 = 0x100000000000000000000000000000000)
    | _  -> ()
 
-/// Specs
-///
-/// Note: lacking any type of functors for F*, this is a copy/paste of [FStar.Int.fst], where the relevant bits that changed are:
-///  - definition of max and min
-///  - use of regular integer modulus instead of wrap-around modulus
-
-let max_int (n:nat) : Tot int = pow2 n - 1
-let min_int (n:nat) : Tot int = 0
-
-let fits (x:int) (n:nat) : Tot bool = min_int n <= x && x <= max_int n
-let size (x:int) (n:nat) : Tot Type0 = b2t(fits x n)
-
-(* Machine integer type *)
-type uint_t (n:nat) = x:int{size x n}
-
-/// Constants
-
-val zero: n:nat -> Tot (uint_t n)
-let zero n = 0
-
-#push-options "--initial_fuel 1 --max_fuel 1"
-
-val pow2_n: #n:pos -> p:nat{p < n} -> Tot (uint_t n)
-let pow2_n #n p = pow2_le_compat (n - 1) p; pow2 p
-
-val one: n:pos -> Tot (uint_t n)
-let one n = 1
-
-#pop-options
-
-val ones: n:nat -> Tot (uint_t n)
-let ones n = max_int n
-
-(* Increment and decrement *)
-val incr: #n:nat -> a:uint_t n -> Pure (uint_t n)
-  (requires (b2t (a < max_int n))) (ensures (fun _ -> True))
-let incr #n a = a + 1
-
-val decr: #n:nat -> a:uint_t n -> Pure (uint_t n)
-  (requires (b2t (a > min_int n))) (ensures (fun _ -> True))
-let decr #n a = a - 1
-
-abstract
-val incr_underspec: #n:nat -> a:uint_t n -> Pure (uint_t n)
-  (requires (b2t (a < max_int n)))
-  (ensures (fun b -> a + 1 = b))
 let incr_underspec #n a =
   if a < max_int n then a + 1 else 0
 
-abstract
-val decr_underspec: #n:nat -> a:uint_t n -> Pure (uint_t n)
-  (requires (b2t (a > min_int n)))
-  (ensures (fun b -> a - 1 = b))
 let decr_underspec #n a =
   if a > min_int n then a - 1 else 0
 
-val incr_mod: #n:nat -> a:uint_t n -> Tot (uint_t n)
-let incr_mod #n a = (a + 1) % (pow2 n)
-
-val decr_mod: #n:nat -> a:uint_t n -> Tot (uint_t n)
-let decr_mod #n a = (a - 1) % (pow2 n)
-
-(* Addition primitives *)
-val add: #n:nat -> a:uint_t n -> b:uint_t n -> Pure (uint_t n)
-  (requires (size (a + b) n))
-  (ensures (fun _ -> True))
-let add #n a b = a + b
-
-abstract
-val add_underspec: #n:nat -> a:uint_t n -> b:uint_t n -> Pure (uint_t n)
-  (requires True)
-  (ensures (fun c ->
-    size (a + b) n ==> a + b = c))
 let add_underspec #n a b =
   if fits (a+b) n then a + b else 0
 
-val add_mod: #n:nat -> uint_t n -> uint_t n -> Tot (uint_t n)
-let add_mod #n a b =
-  (a + b) % (pow2 n)
-
-(* Subtraction primitives *)
-val sub: #n:nat -> a:uint_t n -> b:uint_t n -> Pure (uint_t n)
-  (requires (size (a - b) n))
-  (ensures (fun _ -> True))
-let sub #n a b = a - b
-
-abstract val sub_underspec: #n:nat -> a:uint_t n -> b:uint_t n -> Pure (uint_t n)
-  (requires True)
-  (ensures (fun c ->
-    size (a - b) n ==> a - b = c))
 let sub_underspec #n a b =
   if fits (a-b) n then a - b else 0
 
-val sub_mod: #n:nat -> a:uint_t n -> b:uint_t n -> Tot (uint_t n)
-let sub_mod #n a b =
-  (a - b) % (pow2 n)
-
-(* Multiplication primitives *)
-val mul: #n:nat -> a:uint_t n -> b:uint_t n -> Pure (uint_t n)
-  (requires (size (a * b) n))
-  (ensures (fun _ -> True))
-let mul #n a b = a * b
-
-abstract
-val mul_underspec: #n:nat -> a:uint_t n -> b:uint_t n -> Pure (uint_t n)
-  (requires True)
-  (ensures (fun c ->
-    size (a * b) n ==> a * b = c))
 let mul_underspec #n a b =
   if fits (a*b) n then a * b else 0
 
-val mul_mod: #n:nat -> a:uint_t n -> b:uint_t n -> Tot (uint_t n)
-let mul_mod #n a b =
-  (a * b) % (pow2 n)
+#push-options "--fuel 0 --ifuel 0"
+let lt_square_div_lt a b = ()
 
-private
-let lt_square_div_lt (a:nat) (b:pos) : Lemma
-  (requires (a < b * b))
-  (ensures (a / b < b))
-  = ()
-
-val mul_div: #n:nat -> a:uint_t n -> b:uint_t n -> Tot (uint_t n)
-let mul_div #n a b =
-  FStar.Math.Lemmas.lemma_mult_lt_sqr a b (pow2 n);
-  lt_square_div_lt (a * b) (pow2 n);
-  (a * b) / (pow2 n)
-
-(* Division primitives *)
-val div: #n:nat -> a:uint_t n -> b:uint_t n{b <> 0} -> Pure (uint_t n)
-  (requires (size (a / b) n))
-  (ensures (fun c -> b <> 0 ==> a / b = c))
-let div #n a b = a / b
-
-abstract
-val div_underspec: #n:nat -> a:uint_t n -> b:uint_t n{b <> 0} -> Pure (uint_t n)
-  (requires True)
-  (ensures (fun c ->
-    (b <> 0 /\ size (a / b) n) ==> a / b = c))
 let div_underspec #n a b =
   if fits (a / b) n then a / b else 0
+#pop-options
 
-val div_size: #n:pos -> a:uint_t n -> b:uint_t n{b <> 0} ->
-  Lemma (requires (size a n)) (ensures (size (a / b) n))
 let div_size #n a b =
   FStar.Math.Lib.slash_decr_axiom a b; ()
 
-val udiv: #n:pos -> a:uint_t n -> b:uint_t n{b <> 0} ->
-  Tot (c:uint_t n{b <> 0 ==> a / b = c})
-let udiv #n a b =
-  div_size #n a b;
-  a / b
-
-
-(* Modulo primitives *)
-val mod: #n:nat -> a:uint_t n -> b:uint_t n{b <> 0} -> Tot (uint_t n)
-let mod #n a b = a - ((a/b) * b)
-
-(* Comparison operators *)
-let eq #n (a:uint_t n) (b:uint_t n) : Tot bool = (a = b)
-let gt #n (a:uint_t n) (b:uint_t n) : Tot bool = (a > b)
-let gte #n (a:uint_t n) (b:uint_t n) : Tot bool = (a >= b)
-let lt #n (a:uint_t n) (b:uint_t n) : Tot bool = (a < b)
-let lte #n (a:uint_t n) (b:uint_t n) : Tot bool = (a <= b)
-
-/// Casts
-
-#push-options "--initial_fuel 1 --max_fuel 1"
-
-val to_uint_t: m:nat -> a:int -> Tot (uint_t m)
-let to_uint_t m a = a % pow2 m
-
 open FStar.Seq
 
-(* WARNING: Mind the big endian vs little endian definition *)
-
-(* Casts *)
-val to_vec: #n:nat -> num:uint_t n -> Tot (bv_t n)
-let rec to_vec #n num =
-  if n = 0 then Seq.empty #bool
-  else Seq.append (to_vec #(n - 1) (num / 2)) (Seq.create 1 (num % 2 = 1))
-
-val from_vec: #n:nat -> vec:bv_t n -> Tot (uint_t n)
-let rec from_vec #n vec =
-  if n = 0 then 0
-  else 2 * from_vec #(n - 1) (slice vec 0 (n - 1)) + (if index vec (n - 1) then 1 else 0)
-
-val to_vec_lemma_1: #n:nat -> a:uint_t n -> b:uint_t n ->
-  Lemma (requires a = b) (ensures equal (to_vec a) (to_vec b))
 let to_vec_lemma_1 #n a b = ()
 
-val to_vec_lemma_2: #n:nat -> a:uint_t n -> b:uint_t n ->
-  Lemma (requires equal (to_vec a) (to_vec b)) (ensures a = b)
 let rec to_vec_lemma_2 #n a b =
   if n = 0 then () else begin
     assert(equal (slice (to_vec b) 0 (n - 1)) (to_vec #(n - 1) (b / 2)));
@@ -253,55 +74,32 @@ let rec to_vec_lemma_2 #n a b =
     assert(a % 2 = b % 2)
   end
 
-val inverse_aux: #n:nat -> vec:bv_t n -> i:nat{i < n} ->
-  Lemma (requires True) (ensures index vec i = index (to_vec (from_vec vec)) i)
-        [SMTPat (index (to_vec (from_vec vec)) i)]
 let rec inverse_aux #n vec i =
   if i = n - 1 then
     assert((from_vec vec) % 2 = (if index vec (n - 1) then 1 else 0))
   else inverse_aux #(n - 1) (slice vec 0 (n - 1)) i
 
-val inverse_vec_lemma: #n:nat -> vec:bv_t n ->
-  Lemma (requires True) (ensures equal vec (to_vec (from_vec vec)))
-        [SMTPat (to_vec (from_vec vec))]
 let inverse_vec_lemma #n vec = ()
 
-val inverse_num_lemma: #n:nat -> num:uint_t n ->
-  Lemma (requires True) (ensures num = from_vec (to_vec num))
-        [SMTPat (from_vec (to_vec num))]
 let inverse_num_lemma #n num = to_vec_lemma_2 #n num (from_vec (to_vec num))
 
-val from_vec_lemma_1: #n:nat -> a:bv_t n -> b:bv_t n ->
-  Lemma (requires equal a b) (ensures from_vec a = from_vec b)
 let from_vec_lemma_1 #n a b = ()
 
-val from_vec_lemma_2: #n:nat -> a:bv_t n -> b:bv_t n ->
-  Lemma (requires from_vec a = from_vec b) (ensures equal a b)
 let from_vec_lemma_2 #n a b = inverse_vec_lemma a; inverse_vec_lemma b
 
 
 open FStar.Math.Lemmas
 
-#pop-options
-
-val from_vec_aux: #n:nat -> a:bv_t n -> s1:nat{s1 < n} -> s2:nat{s2 < s1} ->
-  Lemma (requires True)
-        (ensures (from_vec #s2 (slice a 0 s2)) * pow2 (n - s2) + (from_vec #(s1 - s2) (slice a s2 s1)) * pow2 (n - s1) + (from_vec #(n - s1) (slice a s1 n)) = ((from_vec #s2 (slice a 0 s2)) * pow2 (s1 - s2) + (from_vec #(s1 - s2) (slice a s2 s1))) * pow2 (n - s1) + (from_vec #(n - s1) (slice a s1 n)))
+#push-options "--fuel 0 --ifuel 0"
 let from_vec_aux #n a s1 s2 =
   paren_mul_left (from_vec #s2 (slice a 0 s2)) (pow2 (s1 - s2)) (pow2 (n - s1));
   paren_mul_right (from_vec #s2 (slice a 0 s2)) (pow2 (s1 - s2)) (pow2 (n - s1));
   pow2_plus (s1 - s2) (n - s1)
+#pop-options
 
-val seq_slice_lemma: #n:nat -> a:bv_t n -> s1:nat{s1 < n} -> t1:nat{t1 >= s1 && t1 <= n} -> s2:nat{s2 < t1 - s1} -> t2:nat{t2 >= s2 && t2 <= t1 - s1} ->
-  Lemma (equal (slice (slice a s1 t1) s2 t2) (slice a (s1 + s2) (s1 + t2)))
 let seq_slice_lemma #n a s1 t1 s2 t2 = ()
 
 #push-options "--initial_fuel 1 --max_fuel 1"
-
-val from_vec_propriety: #n:pos -> a:bv_t n -> s:nat{s < n} ->
-  Lemma (requires True)
-        (ensures from_vec a = (from_vec #s (slice a 0 s)) * pow2 (n - s) + from_vec #(n - s) (slice a s n))
-        (decreases (n - s))
 let rec from_vec_propriety #n a s =
   if s = n - 1 then () else begin
     from_vec_propriety #n a (s + 1);
@@ -313,197 +111,80 @@ let rec from_vec_propriety #n a s =
     seq_slice_lemma #n a s n 0 1;
     seq_slice_lemma #n a s n 1 (n - s)
   end
-
 #pop-options
 
-val append_lemma: #n:pos -> #m:pos -> a:bv_t n -> b:bv_t m ->
-  Lemma (from_vec #(n + m) (append a b) = (from_vec #n a) * pow2 m + (from_vec #m b))
 let append_lemma #n #m a b =
   assert(equal a (slice (append a b) 0 n));
   assert(equal b (slice (append a b) n (n + m)));
   from_vec_propriety #(n + m) (append a b) n
 
-val slice_left_lemma: #n:pos -> a:bv_t n -> s:pos{s < n} ->
-  Lemma (requires True)
-        (ensures from_vec #s (slice a 0 s) = (from_vec #n a) / (pow2 (n - s)))
 let slice_left_lemma #n a s =
   from_vec_propriety #n a s;
   division_addition_lemma (from_vec #(n - s) (slice a s n)) (pow2 (n - s)) (from_vec #s (slice a 0 s));
   small_division_lemma_1 (from_vec #(n - s) (slice a s n)) (pow2 (n - s))
 
-val slice_right_lemma: #n:pos -> a:bv_t n -> s:pos{s < n} ->
-  Lemma (requires True)
-        (ensures from_vec #s (slice a (n - s) n) = (from_vec #n a) % (pow2 s))
 let slice_right_lemma #n a s =
   from_vec_propriety #n a (n - s);
   modulo_addition_lemma (from_vec #s (slice a (n - s) n)) (pow2 s) (from_vec #(n - s) (slice a 0 (n - s)));
   small_modulo_lemma_1 (from_vec #s (slice a (n - s) n)) (pow2 s)
 
-#push-options "--initial_fuel 1 --max_fuel 1"
-
-(* Relations between constants in BitVector and in UInt. *)
-val zero_to_vec_lemma: #n:pos -> i:nat{i < n} ->
-  Lemma (requires True) (ensures index (to_vec (zero n)) i = index (zero_vec #n) i)
-        [SMTPat (index (to_vec (zero n)) i)]
 let rec zero_to_vec_lemma #n i =
   if i = n - 1 then () else zero_to_vec_lemma #(n - 1) i
 
-val zero_from_vec_lemma: #n:pos ->
-  Lemma (requires True) (ensures from_vec (zero_vec #n) = zero n)
-        [SMTPat (from_vec (zero_vec #n))]
 let zero_from_vec_lemma #n = to_vec_lemma_2 (from_vec (zero_vec #n)) (zero n)
 
-val one_to_vec_lemma: #n:pos -> i:nat{i < n} ->
-  Lemma (requires True)
-        (ensures index (to_vec (one n)) i = index (elem_vec #n (n - 1)) i)
-        [SMTPat (index (to_vec (one n)) i)]
 let one_to_vec_lemma #n i =
   if i = n - 1 then () else zero_to_vec_lemma #n i
 
-val pow2_to_vec_lemma: #n:pos -> p:nat{p < n} -> i:nat{i < n} ->
-  Lemma (requires True)
-        (ensures index (to_vec (pow2_n #n p)) i = index (elem_vec #n (n - p - 1)) i)
-        [SMTPat (index (to_vec (pow2_n #n p)) i)]
 let rec pow2_to_vec_lemma #n p i =
   if i = n - 1 then ()
   else if p = 0 then one_to_vec_lemma #n i
   else pow2_to_vec_lemma #(n - 1) (p - 1) i
 
-val pow2_from_vec_lemma: #n:pos -> p:nat{p < n} ->
-  Lemma (requires True) (ensures from_vec (elem_vec #n p) = pow2_n #n (n - p - 1))
-        [SMTPat (from_vec (elem_vec #n p))]
 let pow2_from_vec_lemma #n p =
   to_vec_lemma_2 (from_vec (elem_vec #n p)) (pow2_n #n (n - p - 1))
 
-val ones_to_vec_lemma: #n:pos -> i:nat{i < n} ->
-  Lemma (requires True)
-        (ensures index (to_vec (ones n)) i = index (ones_vec #n) i)
-        [SMTPat (index (to_vec (ones n)) i)]
 let rec ones_to_vec_lemma #n i =
   if i = n - 1 then () else ones_to_vec_lemma #(n - 1) i
 
-val ones_from_vec_lemma: #n:pos ->
-  Lemma (requires True) (ensures from_vec (ones_vec #n) = ones n)
-        [SMTPat (from_vec (ones_vec #n))]
 let ones_from_vec_lemma #n =
   to_vec_lemma_2 (from_vec (ones_vec #n)) (ones n)
 
-
-(* (nth a i) returns a boolean indicating the i-th bit of a. *)
-val nth: #n:pos -> a:uint_t n -> i:nat{i < n} -> Tot bool
-let nth #n a i = index (to_vec #n a) i
-
-val nth_lemma: #n:pos -> a:uint_t n -> b:uint_t n ->
-  Lemma (requires forall (i:nat{i < n}). nth a i = nth b i)
-        (ensures a = b)
 let nth_lemma #n a b =
   assert(forall (i:nat{i < n}). index (to_vec #n a) i = index (to_vec #n b) i);
   to_vec_lemma_2 a b
 
-(* Lemmas for constants *)
-val zero_nth_lemma: #n:pos -> i:nat{i < n} ->
-  Lemma (requires True) (ensures nth (zero n) i = false)
-        [SMTPat (nth (zero n) i)]
 let zero_nth_lemma #n i = ()
 
-val pow2_nth_lemma: #n:pos -> p:nat{p < n} -> i:nat{i < n} ->
-  Lemma (requires True)
-        (ensures (i = n - p - 1 ==> nth (pow2_n #n p) i = true) /\
-                 (i <> n - p - 1 ==> nth (pow2_n #n p) i = false))
-        [SMTPat (nth (pow2_n #n p) i)]
 let pow2_nth_lemma #n p i = ()
 
-val one_nth_lemma: #n:pos -> i:nat{i < n} ->
-  Lemma (requires True)
-        (ensures (i = n - 1 ==> nth (one n) i = true) /\
-                 (i < n - 1 ==> nth (one n) i = false))
-        [SMTPat (nth (one n) i)]
 let one_nth_lemma #n i = ()
 
-val ones_nth_lemma: #n:pos -> i:nat{i < n} ->
-  Lemma (requires True) (ensures (nth (ones n) i) = true)
-        [SMTPat (nth (ones n) i)]
 let ones_nth_lemma #n i = ()
 
-(* Bitwise operators *)
-val logand: #n:pos -> a:uint_t n -> b:uint_t n -> Tot (uint_t n)
-let logand #n a b = from_vec #n (logand_vec #n (to_vec #n a) (to_vec #n b))
-
-val logxor: #n:pos -> a:uint_t n -> b:uint_t n -> Tot (uint_t n)
-let logxor #n a b = from_vec #n (logxor_vec #n (to_vec #n a) (to_vec #n b))
-
-val logor: #n:pos -> a:uint_t n -> b:uint_t n -> Tot (uint_t n)
-let logor #n a b = from_vec #n (logor_vec #n (to_vec #n a) (to_vec #n b))
-
-val lognot: #n:pos -> a:uint_t n  -> Tot (uint_t n)
-let lognot #n a = from_vec #n (lognot_vec #n (to_vec #n a))
-
-(* Bitwise operators definitions *)
-val logand_definition: #n:pos -> a:uint_t n -> b:uint_t n -> i:nat{i < n} ->
-  Lemma (requires True)
-        (ensures (nth (logand a b) i = (nth a i && nth b i)))
-        [SMTPat (nth (logand a b) i)]
 let logand_definition #n a b i = ()
 
-val logxor_definition: #n:pos -> a:uint_t n -> b:uint_t n -> i:nat{i < n} ->
-  Lemma (requires True)
-        (ensures (nth (logxor a b) i = (nth a i <> nth b i)))
-        [SMTPat (nth (logxor a b) i)]
 let logxor_definition #n a b i = ()
 
-val logor_definition: #n:pos -> a:uint_t n -> b:uint_t n -> i:nat{i < n} ->
-  Lemma (requires True)
-        (ensures (nth (logor a b) i = (nth a i || nth b i)))
-        [SMTPat (nth (logor a b) i)]
 let logor_definition #n a b i = ()
 
-val lognot_definition: #n:pos -> a:uint_t n -> i:nat{i < n} ->
-  Lemma (requires True)
-        (ensures (nth (lognot a) i = not(nth a i)))
-        [SMTPat (nth (lognot a) i)]
 let lognot_definition #n a i = ()
 
-(* Two's complement unary minus *)
-inline_for_extraction
-val minus: #n:pos -> a:uint_t n -> Tot (uint_t n)
-let minus #n a = add_mod (lognot a) 1
-
-(* Bitwise operators lemmas *)
-(* TODO: lemmas about the relations between different operators *)
-(* Bitwise AND operator *)
-val logand_commutative: #n:pos -> a:uint_t n -> b:uint_t n ->
-  Lemma (requires True) (ensures (logand #n a b = logand #n b a))
 let logand_commutative #n a b = nth_lemma #n (logand #n a b) (logand #n b a)
 
-val logand_associative: #n:pos -> a:uint_t n -> b:uint_t n -> c:uint_t n ->
-  Lemma (requires True)
-        (ensures (logand #n (logand #n a b) c = logand #n a (logand #n b c)))
 let logand_associative #n a b c = nth_lemma #n (logand #n (logand #n a b) c) (logand #n a (logand #n b c))
 
-val logand_self: #n:pos -> a:uint_t n ->
-  Lemma (requires True) (ensures (logand #n a a = a))
 let logand_self #n a = nth_lemma #n (logand #n a a) a
 
-val logand_lemma_1: #n:pos -> a:uint_t n ->
-  Lemma (requires True) (ensures (logand #n a (zero n) = zero n))
 let logand_lemma_1 #n a = nth_lemma #n (logand #n a (zero n)) (zero n)
 
-val logand_lemma_2: #n:pos -> a:uint_t n ->
-  Lemma (requires True) (ensures (logand #n a (ones n) = a))
 let logand_lemma_2 #n a = nth_lemma #n (logand #n a (ones n)) a
 
-(* subset_vec_le_lemma proves that a subset of bits is numerically smaller or equal. *)
-val subset_vec_le_lemma: #n:pos -> a:bv_t n -> b:bv_t n ->
-  Lemma (requires is_subset_vec #n a b) (ensures (from_vec a) <= (from_vec b))
 let rec subset_vec_le_lemma #n a b = match n with
   | 1 -> ()
   | _ -> lemma_slice_subset_vec #n a b 0 (n-1);
         subset_vec_le_lemma #(n-1) (slice a 0 (n-1)) (slice b 0 (n-1))
 
-(* logand_le proves the the result of AND is less than or equal to both arguments. *)
-val logand_le: #n:pos -> a:uint_t n -> b:uint_t n ->
-  Lemma (requires True)
-        (ensures (logand a b) <= a /\ (logand a b) <= b)
 let logand_le #n a b =
   let va = to_vec a in
   let vb = to_vec b in
@@ -511,38 +192,18 @@ let logand_le #n a b =
   subset_vec_le_lemma #n vand va;
   subset_vec_le_lemma #n vand vb
 
-(* Bitwise XOR operator *)
-val logxor_commutative: #n:pos -> a:uint_t n -> b:uint_t n ->
-  Lemma (requires True) (ensures (logxor #n a b = logxor #n b a))
 let logxor_commutative #n a b = nth_lemma #n (logxor #n a b) (logxor #n b a)
 
-val logxor_associative: #n:pos -> a:uint_t n -> b:uint_t n -> c:uint_t n ->
-  Lemma (requires True) (ensures (logxor #n (logxor #n a b) c = logxor #n a (logxor #n b c)))
 let logxor_associative #n a b c = nth_lemma #n (logxor #n (logxor #n a b) c) (logxor #n a (logxor #n b c))
 
-val logxor_self: #n:pos -> a:uint_t n ->
-  Lemma (requires True) (ensures (logxor #n a a = zero n))
 let logxor_self #n a = nth_lemma #n (logxor #n a a) (zero n)
 
-val logxor_lemma_1: #n:pos -> a:uint_t n ->
-  Lemma (requires True) (ensures (logxor #n a (zero n) = a))
 let logxor_lemma_1 #n a = nth_lemma #n (logxor #n a (zero n)) a
 
-val logxor_lemma_2: #n:pos -> a:uint_t n ->
-  Lemma (requires True) (ensures (logxor #n a (ones n) = lognot #n a))
 let logxor_lemma_2 #n a = nth_lemma #n (logxor #n a (ones n)) (lognot #n a)
 
-#reset-options "--initial_fuel 0 --max_fuel 0"
+let xor_lemma _ _ = ()
 
-private let xor (b:bool) (b':bool) : Tot bool = b <> b'
-private let xor_lemma (a:bool) (b:bool) : Lemma
-  (requires (True))
-  (ensures  (xor (xor a b) b = a))
-  [SMTPat (xor (xor a b) b)]
-  = ()
-
-val logxor_inv: #n:pos -> a:uint_t n -> b:uint_t n -> Lemma
-  (a = logxor #n (logxor #n a b) b)
 let logxor_inv #n a b =
   let open FStar.BitVector in
   let open FStar.Seq in
@@ -557,8 +218,6 @@ let logxor_inv #n a b =
   Seq.lemma_eq_intro (logxor_vec (logxor_vec va vb) vb) va;
   inverse_num_lemma a; inverse_num_lemma b
 
-val logxor_neq_nonzero: #n:pos -> a:uint_t n -> b:uint_t n -> Lemma
-   (a <> b ==> logxor a b <> 0)
 let logxor_neq_nonzero #n a b =
   let va = to_vec a in
   let vb = to_vec b in
@@ -572,43 +231,21 @@ let logxor_neq_nonzero #n a b =
     assert (from_vec va = from_vec vb)
   end
 
-(* Bitwise OR operators *)
-val logor_commutative: #n:pos -> a:uint_t n -> b:uint_t n ->
-  Lemma (requires True) (ensures (logor #n a b = logor #n b a))
 let logor_commutative #n a b = nth_lemma #n (logor #n a b) (logor #n b a)
 
-val logor_associative: #n:pos -> a:uint_t n -> b:uint_t n -> c:uint_t n ->
-  Lemma (requires True)
-        (ensures (logor #n (logor #n a b) c = logor #n a (logor #n b c)))
 let logor_associative #n a b c = nth_lemma #n (logor #n (logor #n a b) c) (logor #n a (logor #n b c))
 
-val logor_self: #n:pos -> a:uint_t n ->
-  Lemma (requires True) (ensures (logor #n a a = a))
 let logor_self #n a = nth_lemma #n (logor #n a a) a
 
-val logor_lemma_1: #n:pos -> a:uint_t n ->
-  Lemma (requires True) (ensures (logor #n a (zero n) = a))
 let logor_lemma_1 #n a = nth_lemma (logor #n a (zero n)) a
 
-val logor_lemma_2: #n:pos -> a:uint_t n ->
-  Lemma (requires True) (ensures (logor #n a (ones n) = ones n))
 let logor_lemma_2 #n a = nth_lemma (logor #n a (ones n)) (ones n)
 
-#set-options "--initial_fuel 1 --max_fuel 1"
-
-(* superset_vec_le_lemma proves that a superset of bits is numerically greater than or equal. *)
-val superset_vec_ge_lemma: #n:pos -> a:bv_t n -> b:bv_t n ->
-  Lemma (requires is_superset_vec #n a b)
-        (ensures (from_vec a) >= (from_vec b))
 let rec superset_vec_ge_lemma #n a b = match n with
   | 1 -> ()
   | _ -> lemma_slice_superset_vec #n a b 0 (n-1);
         superset_vec_ge_lemma #(n-1) (slice a 0 (n-1)) (slice b 0 (n-1))
 
-(* logor_ge proves that the result of an OR is greater than or equal to both arguments. *)
-val logor_ge: #n:pos -> a:uint_t n -> b:uint_t n ->
-  Lemma (requires True)
-        (ensures (logor a b) >= a /\ (logor a b) >= b)
 let logor_ge #n a b =
   let va = to_vec a in
   let vb = to_vec b in
@@ -616,20 +253,10 @@ let logor_ge #n a b =
   superset_vec_ge_lemma #n vor va;
   superset_vec_ge_lemma #n vor vb
 
-(* Bitwise NOT operator *)
-val lognot_self: #n:pos -> a:uint_t n ->
-  Lemma (requires True) (ensures (lognot #n (lognot #n a) = a))
 let lognot_self #n a = nth_lemma (lognot #n (lognot #n a)) a
 
-val lognot_lemma_1: #n:pos ->
-  Lemma (requires True) (ensures (lognot #n (zero n) = ones n))
 let lognot_lemma_1 #n = nth_lemma (lognot #n (zero n)) (ones n)
 
-(** Used in the next two lemmas *)
-private val to_vec_mod_pow2: #n:nat -> a:uint_t n -> m:pos -> i:nat{n - m <= i /\ i < n} ->
-  Lemma (requires (a % pow2 m == 0))
-        (ensures  (index (to_vec a) i == false))
-        [SMTPat (index (to_vec #n a) i); SMTPat (a % pow2 m == 0)]
 let rec to_vec_mod_pow2 #n a m i =
   if i = n - 1 then
     begin
@@ -644,11 +271,6 @@ let rec to_vec_mod_pow2 #n a m i =
     to_vec_mod_pow2 #(n - 1) (a / 2) (m - 1) i
     end
 
-(** Used in the next two lemmas *)
-private val to_vec_lt_pow2: #n:nat -> a:uint_t n -> m:nat -> i:nat{i < n - m} ->
-  Lemma (requires (a < pow2 m))
-        (ensures  (index (to_vec a) i == false))
-        [SMTPat (index (to_vec #n a) i); SMTPat (a < pow2 m)]
 let rec to_vec_lt_pow2 #n a m i =
   if n = 0 then ()
   else
@@ -662,13 +284,7 @@ let rec to_vec_lt_pow2 #n a m i =
       end
 
 (** Used in the next two lemmas *)
-#reset-options "--initial_fuel 0 --max_fuel 1 --z3rlimit 40"
-private val index_to_vec_ones: #n:pos -> m:nat{m <= n} -> i:nat{i < n} ->
-  Lemma (requires True)
-        (ensures (pow2 m <= pow2 n /\
-          (i < n - m ==> index (to_vec #n (pow2 m - 1)) i == false) /\
-          (n - m <= i ==> index (to_vec #n (pow2 m - 1)) i == true)))
-        [SMTPat (index (to_vec #n (pow2 m - 1)) i)]
+#push-options "--initial_fuel 0 --max_fuel 1 --z3rlimit 40"
 let rec index_to_vec_ones #n m i =
    let a = pow2 m - 1 in
    pow2_le_compat n m;
@@ -676,12 +292,8 @@ let rec index_to_vec_ones #n m i =
    else if m = n then ones_to_vec_lemma #n i
    else if i = n - 1 then ()
    else index_to_vec_ones #(n - 1) (m - 1) i
+#pop-options
 
-#reset-options "--initial_fuel 0 --max_fuel 0"
-
-val logor_disjoint: #n:pos -> a:uint_t n -> b:uint_t n -> m:pos{m < n} ->
-  Lemma (requires (a % pow2 m == 0 /\ b < pow2 m))
-        (ensures  (logor #n a b == a + b))
 let logor_disjoint #n a b m =
   assert (a % pow2 m == 0); // To trigger pattern above
   assert (forall (i:nat{n - m <= i /\ i < n}).{:pattern (index (to_vec a) i)}
@@ -701,8 +313,6 @@ let logor_disjoint #n a b m =
   small_modulo_lemma_1 b (pow2 m);
   assert (from_vec #m (slice (to_vec b) (n - m) n) == b)
 
-val logand_mask: #n:pos -> a:uint_t n -> m:pos{m < n} ->
-  Lemma (pow2 m < pow2 n /\ logand #n a (pow2 m - 1) == a % pow2 m)
 let logand_mask #n a m =
   pow2_lt_compat n m;
   Seq.lemma_split (logand_vec (to_vec a) (to_vec (pow2 m - 1))) (n - m);
@@ -715,147 +325,64 @@ let logand_mask #n a m =
   slice_right_lemma #n (to_vec a) m;
   assert (from_vec #m (slice (to_vec a) (n - m) n) == a % pow2 m)
 
-
-(* Shift operators *)
-
-val shift_left: #n:pos -> a:uint_t n -> s:nat -> Tot (uint_t n)
-let shift_left #n a s = from_vec (shift_left_vec #n (to_vec #n a) s)
-
-val shift_right: #n:pos -> a:uint_t n -> s:nat -> Tot (uint_t n)
-let shift_right #n a s = from_vec (shift_right_vec #n (to_vec #n a) s)
-
-(* Shift operators lemmas *)
-val shift_left_lemma_1: #n:pos -> a:uint_t n -> s:nat -> i:nat{i < n && i >= n - s} ->
-  Lemma (requires True)
-        (ensures (nth (shift_left #n a s) i = false))
-        [SMTPat (nth (shift_left #n a s) i)]
 let shift_left_lemma_1 #n a s i = ()
 
-val shift_left_lemma_2: #n:pos -> a:uint_t n -> s:nat -> i:nat{i < n && i < n - s} ->
-  Lemma (requires True)
-        (ensures (nth (shift_left #n a s) i = nth #n a (i + s)))
-        [SMTPat (nth (shift_left #n a s) i)]
 let shift_left_lemma_2 #n a s i = ()
 
-val shift_right_lemma_1: #n:pos -> a:uint_t n -> s:nat -> i:nat{i < n && i < s} ->
-  Lemma (requires True)
-        (ensures (nth (shift_right #n a s) i = false))
-        [SMTPat (nth (shift_right #n a s) i)]
 let shift_right_lemma_1 #n a s i = ()
 
-val shift_right_lemma_2: #n:pos -> a:uint_t n -> s:nat -> i:nat{i < n && i >= s} ->
-  Lemma (requires True)
-        (ensures (nth (shift_right #n a s) i = nth #n a (i - s)))
-        [SMTPat (nth (shift_right #n a s) i)]
 let shift_right_lemma_2 #n a s i = ()
 
-(* Lemmas with shift operators and bitwise operators *)
-val shift_left_logand_lemma: #n:pos -> a:uint_t n -> b:uint_t n -> s:nat ->
-  Lemma (requires True)
-        (ensures (shift_left #n (logand #n a b) s = logand #n (shift_left #n a s) (shift_left #n b s)))
 let shift_left_logand_lemma #n a b s = nth_lemma (shift_left #n (logand #n a b) s) (logand #n (shift_left #n a s) (shift_left #n b s))
 
-val shift_right_logand_lemma: #n:pos -> a:uint_t n -> b:uint_t n -> s:nat ->
-  Lemma (requires True)
-        (ensures (shift_right #n (logand #n a b) s = logand #n (shift_right #n a s) (shift_right #n b s)))
 let shift_right_logand_lemma #n a b s = nth_lemma (shift_right #n (logand #n a b) s) (logand #n (shift_right #n a s) (shift_right #n b s))
 
-val shift_left_logxor_lemma: #n:pos -> a:uint_t n -> b:uint_t n -> s:nat ->
-  Lemma (requires True)
-        (ensures (shift_left #n (logxor #n a b) s = logxor #n (shift_left #n a s) (shift_left #n b s)))
 let shift_left_logxor_lemma #n a b s = nth_lemma (shift_left #n (logxor #n a b) s) (logxor #n (shift_left #n a s) (shift_left #n b s))
 
-val shift_right_logxor_lemma: #n:pos -> a:uint_t n -> b:uint_t n -> s:nat ->
-  Lemma (requires True)
-        (ensures (shift_right #n (logxor #n a b) s = logxor #n (shift_right #n a s) (shift_right #n b s)))
 let shift_right_logxor_lemma #n a b s = nth_lemma (shift_right #n (logxor #n a b) s) (logxor #n (shift_right #n a s) (shift_right #n b s))
 
-val shift_left_logor_lemma: #n:pos -> a:uint_t n -> b:uint_t n -> s:nat ->
-  Lemma (requires True)
-        (ensures (shift_left #n (logor #n a b) s = logor #n (shift_left #n a s) (shift_left #n b s)))
 let shift_left_logor_lemma #n a b s = nth_lemma (shift_left #n (logor #n a b) s) (logor #n (shift_left #n a s) (shift_left #n b s))
 
-val shift_right_logor_lemma: #n:pos -> a:uint_t n -> b:uint_t n -> s:nat ->
-  Lemma (requires True)
-        (ensures (shift_right #n (logor #n a b) s = logor #n (shift_right #n a s) (shift_right #n b s)))
 let shift_right_logor_lemma #n a b s = nth_lemma (shift_right #n (logor #n a b) s) (logor #n (shift_right #n a s) (shift_right #n b s))
 
 
-(* Lemmas about value after shift operations *)
-val shift_left_value_aux_1: #n:pos -> a:uint_t n -> s:nat{s >= n} ->
-  Lemma (requires True)
-        (ensures shift_left #n a s = (a * pow2 s) % pow2 n)
 let shift_left_value_aux_1 #n a s = pow2_multiplication_modulo_lemma_1 a n s
 
-val shift_left_value_aux_2: #n:pos -> a:uint_t n ->
-  Lemma (requires True)
-        (ensures shift_left #n a 0 = (a * pow2 0) % pow2 n)
 let shift_left_value_aux_2 #n a =
   assert_norm(a * pow2 0 = a);
   small_modulo_lemma_1 a (pow2 n)
 
-val shift_left_value_aux_3: #n:pos -> a:uint_t n -> s:pos{s < n} ->
-  Lemma (requires True)
-        (ensures shift_left #n a s = (a * pow2 s) % pow2 n)
 let shift_left_value_aux_3 #n a s =
   append_lemma #(n - s) #s (slice (to_vec a) s n) (zero_vec #s);
   slice_right_lemma #n (to_vec a) (n - s);
   pow2_multiplication_modulo_lemma_2 a n s
 
-val shift_left_value_lemma: #n:pos -> a:uint_t n -> s:nat ->
-  Lemma (requires True)
-        (ensures shift_left #n a s = (a * pow2 s) % pow2 n)
-        [SMTPat (shift_left #n a s)]
 let shift_left_value_lemma #n a s =
   if s >= n then shift_left_value_aux_1 #n a s
   else if s = 0 then shift_left_value_aux_2 #n a
   else shift_left_value_aux_3 #n a s
 
-val shift_right_value_aux_1: #n:pos -> a:uint_t n -> s:nat{s >= n} ->
-  Lemma (requires True)
-        (ensures shift_right #n a s = a / pow2 s)
 let shift_right_value_aux_1 #n a s =
   pow2_le_compat s n;
   small_division_lemma_1 a (pow2 s)
 
-val shift_right_value_aux_2: #n:pos -> a:uint_t n ->
-  Lemma (requires True)
-        (ensures shift_right #n a 0 = a / pow2 0)
 let shift_right_value_aux_2 #n a = assert_norm (pow2 0 == 1)
 
-val shift_right_value_aux_3: #n:pos -> a:uint_t n -> s:pos{s < n} ->
-  Lemma (requires True)
-        (ensures shift_right #n a s = a / pow2 s)
 let shift_right_value_aux_3 #n a s =
   append_lemma #s #(n - s) (zero_vec #s) (slice (to_vec a) 0 (n - s));
   slice_left_lemma #n (to_vec a) (n - s)
 
-val shift_right_value_lemma: #n:pos -> a:uint_t n -> s:nat ->
-  Lemma (requires True)
-        (ensures shift_right #n a s = a / pow2 s)
-        [SMTPat (shift_right #n a s)]
 let shift_right_value_lemma #n a s =
   if s >= n then shift_right_value_aux_1 #n a s
   else if s = 0 then shift_right_value_aux_2 #n a
   else shift_right_value_aux_3 #n a s
 
-
-(* Lemmas about the most significant bit in various situations *)
-
-val msb: #n:pos -> a:uint_t n -> Tot bool
-let msb #n a = nth a 0
-
-#set-options "--initial_fuel 1 --max_fuel 1"
-val lemma_msb_pow2: #n:pos -> a:uint_t n ->
-  Lemma (msb a <==> a >= pow2 (n-1))
 let lemma_msb_pow2 #n a = if n = 1 then () else from_vec_propriety (to_vec a) 1
 
-private val plus_one_mod : p:pos -> a:nat ->
+val plus_one_mod : p:pos -> a:nat ->
     Lemma (requires (a < p /\ ((a + 1) % p == 0))) (ensures (a == p - 1))
-private let plus_one_mod p a = ()
+let plus_one_mod p a = ()
 
-val lemma_minus_zero: #n:pos -> a:uint_t n ->
-  Lemma (minus a = 0 ==> a = 0)
 let lemma_minus_zero #n a =
   if minus a = 0 then
   begin
@@ -865,25 +392,20 @@ let lemma_minus_zero #n a =
     logxor_lemma_2 #n (ones n)
   end
 
-val lemma_msb_gte: #n:pos{n > 1} -> a:uint_t n -> b:uint_t n ->
-  Lemma ((a >= b && not (msb a)) ==> not (msb b))
+#push-options "--z3rlimit 20 --fuel 1 --ifuel 0"
 let lemma_msb_gte #n a b =
   from_vec_propriety (to_vec a) 1;
   from_vec_propriety (to_vec b) 1
-
+#pop-options
 
 (* Lemmas toward showing ~n + 1 = -a *)
 
-#set-options "--initial_fuel 1 --max_fuel 1 --initial_ifuel 1 --max_ifuel 1"
+// #set-options "--initial_fuel 1 --max_fuel 1 --initial_ifuel 1 --max_ifuel 1"
 
-#set-options "--z3rlimit 80"
-val lemma_uint_mod: #n:pos -> a:uint_t n ->
-  Lemma (a = a % pow2 n)
+#push-options "--z3rlimit 80"
 let lemma_uint_mod #n a = ()
-#set-options "--z3rlimit 5"
+#pop-options
 
-val lemma_add_sub_cancel: #n:pos -> a:uint_t n -> b:uint_t n ->
-  Lemma (add_mod (sub_mod a b) b = a)
 let lemma_add_sub_cancel #n a b =
   let ab = (a-b) % pow2 n in
   let abb = (ab + b) % pow2 n in
@@ -898,15 +420,11 @@ let lemma_add_sub_cancel #n a b =
   assert (((a-b) + b) % p = (((a-b) % p) + b) % p);
   assert (a % p = (((a-b) % p) + b) % p)
 
-val lemma_mod_sub_distr_l: a:int -> b:int -> p:pos ->
-  Lemma ((a - b) % p = ((a % p) - b) % p)
 let lemma_mod_sub_distr_l a b p =
   let q = (a - (a % p)) / p in
   FStar.Math.Lemmas.lemma_mod_spec2 a p;
   FStar.Math.Lemmas.lemma_mod_plus (a % p - b) q p
 
-val lemma_sub_add_cancel: #n:pos -> a:uint_t n -> b:uint_t n ->
-  Lemma (sub_mod (add_mod a b) b = a)
 let lemma_sub_add_cancel #n a b =
   let ab = (a+b) % pow2 n in
   let abb = (ab - b) % pow2 n in
@@ -916,15 +434,6 @@ let lemma_sub_add_cancel #n a b =
   lemma_uint_mod a;
   lemma_mod_sub_distr_l (a+b) b p
 
-let zero_extend_vec (#n:pos) (a:BitVector.bv_t n): Tot (BitVector.bv_t (n+1)) = Seq.append (Seq.create 1 false) a
-let one_extend_vec (#n:pos) (a:BitVector.bv_t n): Tot (BitVector.bv_t (n+1)) = Seq.append (Seq.create 1 true) a
-
-let zero_extend (#n:pos) (a:uint_t n): Tot (uint_t (n+1)) = from_vec (zero_extend_vec (to_vec a))
-let one_extend (#n:pos) (a:uint_t n): Tot (uint_t (n+1)) = from_vec (one_extend_vec (to_vec a))
-
-val lemma_zero_extend: #n:pos -> a:uint_t n ->
-  Lemma (zero_extend a = a)
-  [SMTPat (zero_extend a)]
 let lemma_zero_extend #n a =
   let hd0 = Seq.create 1 false in
   let av = to_vec a in
@@ -935,9 +444,6 @@ let lemma_zero_extend #n a =
   from_vec_propriety #(n+1) eav 1;
   assert (r = a)
 
-val lemma_one_extend: #n:pos -> a:uint_t n ->
-  Lemma (one_extend a = pow2 n + a)
-  [SMTPat (one_extend a)]
 let lemma_one_extend #n a =
   let hd1 = Seq.create 1 true in
   let av = to_vec a in
@@ -948,8 +454,7 @@ let lemma_one_extend #n a =
   from_vec_propriety #(n+1) eav 1;
   assert (r = pow2 n + a)
 
-val lemma_lognot_zero_ext: #n:pos -> a:uint_t n ->
-  Lemma (lognot #(n+1) (zero_extend a) = pow2 n + (lognot #n a))
+#push-options "--fuel 1 --ifuel 0"
 let lemma_lognot_zero_ext #n a =
   let lhs = lognot #(n+1) a in
   let rhs = pow2 n + (lognot #n a) in
@@ -981,9 +486,6 @@ let lemma_lognot_zero_ext #n a =
   assert (neav_l = neav_r);
   assert (from_vec neav_r = lhs)
 
-#set-options "--z3rlimit 20"
-val lemma_lognot_one_ext: #n:pos -> a:uint_t n ->
-  Lemma (lognot #(n+1) (one_extend a) = lognot #n a)
 let lemma_lognot_one_ext #n a =
   let lhs = lognot #(n+1) (one_extend a) in
   let rhs = lognot #n a in
@@ -1000,11 +502,6 @@ let lemma_lognot_one_ext #n a =
   let neav_l = Seq.append hd0 nav in
   Seq.Base.lemma_eq_elim neav_l neav_r
 
-val lemma_lognot_value_mod: #n:pos -> a:uint_t n ->
-  Lemma
-  (requires True)
-  (ensures (lognot a = pow2 n - a - 1))
-  (decreases n)
 let rec lemma_lognot_value_mod #n a =
     if n = 1 then () else
     begin
@@ -1042,8 +539,6 @@ let rec lemma_lognot_value_mod #n a =
       end
     end
 
-val lemma_lognot_value_zero: #n:pos -> a:uint_t n{a = 0} ->
-  Lemma (lognot a = sub_mod (sub_mod 0 a) 1)
 let lemma_lognot_value_zero #n a =
   let p = pow2 n in
   calc (==) {
@@ -1063,6 +558,7 @@ let lemma_lognot_value_zero #n a =
     == { lemma_lognot_value_mod a }
     lognot a;
   }
+#pop-options
 
 #push-options "--z3rlimit 150"
 private
@@ -1071,11 +567,7 @@ val lemma_mod_variation: #n:pos -> a:uint_t n ->
 let lemma_mod_variation #n a = ()
 #pop-options
 
-#push-options "--z3rlimit 5"
-val lemma_one_mod_pow2: #n:pos ->
-  Lemma (1 = 1 % (pow2 n))
 let lemma_one_mod_pow2 #n = ()
-#pop-options
 
 #push-options "--z3rlimit 50"
 private
@@ -1096,8 +588,6 @@ let lemma_lognot_value_variation #n a =
   }
 #pop-options
 
-val lemma_lognot_value_nonzero: #n:pos -> a:uint_t n{a <> 0} ->
-  Lemma (lognot a = sub_mod (sub_mod 0 a) 1)
 let lemma_lognot_value_nonzero #n a =
   let p = pow2 n in
   lemma_lognot_value_variation #n a;
@@ -1107,14 +597,10 @@ let lemma_lognot_value_nonzero #n a =
   assert (((-a) % p) - 1 % p = (((-a) % p) - 1) % p);
   assert ((-a) % p - 1 % p = (((0 - a) % p) - 1) % p)
 
-val lemma_lognot_value: #n:pos -> a:uint_t n ->
-  Lemma (lognot #n a = sub_mod (sub_mod 0 a) 1)
 let lemma_lognot_value #n a =
   if a = 0 then lemma_lognot_value_zero a
   else lemma_lognot_value_nonzero a
 
-val lemma_minus_eq_zero_sub: #n:pos -> a:uint_t n ->
-  Lemma (minus #n a = sub_mod #n 0 a)
 let lemma_minus_eq_zero_sub #n a =
   let na = lognot a in
   let ma = minus a in
